examples/sgx/Test.fst
@@ -1,30 +1,53 @@
 module Test
 open Ast
 
-(*
-  let mylambda = [("main", Seq (1200uL, [(Assign (1200uL, (Register "rbx"), (Constant 1400uL)))]))]
-  let mylambda = [("main", Seq (1200uL, [(Assign (1200uL, (Register "rbx"), (Constant 1400uL)));(Store (1201uL, 1uL, (Register "rbx"), (Constant 10uL)))]))]
- *)
-
  (*
+	Calling Convention:
+	1. First four arguments are sent via rcx, rdx, r8 and r9
+	2. Remaining arguments are sent via stack
+	
+
+ In the below example, we are using only stack (but not heap because bitmap for heap should be set by V)
+
  main:
+
+  rbp := 2100
+  push rbp
   rbp := rsp
-  rbx := 1400uL
-  store rbx 10uL 
-  rdx := load(rbx)
+
+  rbx := 10uL
+  push rbx 
+
+  rbx := 1300uL
+  sub rax rsp rbx  
+  div rcx rax 64uL
+  mod rax rax 64uL
+  add rbx rbx rcx
+  load rcx rbx
+  lsr rax 1uL rax
+  lor rax rcx rax
+  store rbx rax 
   rcx := 0
+  rdx := 0
+  r8 := 0
+  r9 := 0
+
   call "foo"
   rsp := rbp
   return
 
  counter:
+    push rbp
     rbp := rsp
+    add rbx rsp 2uL 
+    load rdx rbx
+
  L1: add rcx rcx 1
     cmp flag rdx rcx
     if flag = 1 then 
       rax := rcx
       jump L2 
-   else
+    else
       jump L1
  L2: rsp := rbp
      return 
@@ -32,37 +55,52 @@ open Ast
 
   let mylambda = [
 		 ("main", 
-		 Seq (1200uL, [(Assign (1200uL, (Register "rbp"), (Constant 1000uL)));(Push (1200uL, (Register "rbp")));
-				(Assign (1201uL, (Register "rbp"), (Register "rsp")));
-				(Assign (1202uL, (Register "rbx"), (Constant 1402uL)));
-		 		(Store (1203uL, 1uL, (Register "rbx"), (Constant 10uL)));
-				(Load (1204uL, (Register "rdx"), 1uL, (Register "rbx")));
-				(Call (1205uL, (Constant 1210uL)));
-		 		(Assign (1206uL, (Register "rsp"), (Register "rbp")));
-				(Pop (1207uL, (Register "rbp")));
-				(Return 1208uL)	
+		 Seq (1200uL, [(Assign (1200uL, (Register "rbp"), (Constant 2100uL)));
+				(Push (1201uL, (Register "rbp")));
+				(Assign (1202uL, (Register "rbp"), (Register "rsp")));
+				(Assign (1203uL, (Register "rbx"), (Constant 10uL)));
+		 		(Push (1204uL, (Register "rbx")));
+				(Assign (1205uL, (Register "rbx"), (Constant 1300uL)));
+				(Sub (1206uL, (Register "rax"), (Register "rsp"),  (Register "rbx")));
+				(Div (1207uL, (Register "rcx"), (Register "rax"),  (Constant 64uL)));
+				(Mod (1208uL, (Register "rax"), (Register "rax"),  (Constant 64uL)));
+				(Add (1209uL, (Register "rbx"), (Register "rbx"),  (Register "rcx")));
+				(Load (1210uL, (Register "rcx"), 1uL, (Register "rbx")));
+				(Lsr (1211uL, (Register "rax"), (Constant 1uL), (Register "rax")));
+				(Lor (1212uL, (Register "rax"), (Register "rcx"), (Register "rax")));
+				(Store (1213uL, 1uL, (Register "rbx"), (Register "rax")));
+				(Assign (1214uL, (Register "rcx"), (Constant 0uL)));
+				(Assign (1215uL, (Register "rdx"), (Constant 0uL)));
+				(Assign (1216uL, (Register "r8"), (Constant 0uL)));
+				(Assign (1217uL, (Register "r9"), (Constant 0uL)));
+				(Call (1218uL, (Constant 1230uL)));
+		 		(Assign (1219uL, (Register "rsp"), (Register "rbp")));
+				(Pop (1220uL, (Register "rbp")));
+				(Return 1221uL)	
 				]));
 		("counter", 
-		 Seq (1210uL, [(Push (1210uL, (Register "rbp")));
-				(Assign (1211uL, (Register "rbp"), (Register "rsp")));
-				(Add (1212uL, (Register "rcx"), (Register "rcx"),(Constant 1uL)));
-				(Cmp (1213uL, (Register "flag"), (Register "rdx"),(Register "rcx")));
-		 		(If (1214uL, (Register "flag"), Seq (1215uL, [  
-						(Assign (1215uL, (Register "rax"), (Register "rcx")));
-						(Jump (1216uL, (Constant 1218uL) ))
+		 Seq (1230uL, [(Push (1230uL, (Register "rbp")));
+				(Assign (1231uL, (Register "rbp"), (Register "rsp")));
+				(Add (1232uL, (Register "rbx"), (Register "rsp"),(Constant 2uL)));
+				(Load (1233uL, (Register "rdx"), 1uL, (Register "rbx")));
+				(Add (1234uL, (Register "rcx"), (Register "rcx"),(Constant 1uL)));
+				(Cmp (1235uL, (Register "flag"), (Register "rdx"),(Register "rcx")));
+		 		(If (1236uL, (Register "flag"), Seq (1237uL, [  
+						(Assign (1237uL, (Register "rax"), (Register "rcx")));
+						(Jump (1238uL, (Constant 1240uL) ))
 						 ]),
-					     Seq (1217uL, [  
-						(Jump (1217uL, (Constant 1212uL) ))
+					     Seq (1239uL, [  
+						(Jump (1239uL, (Constant 1234uL) ))
 						 ])
 				    )
 				);
-		 		(Assign (1218uL, (Register "rsp"), (Register "rbp")));
-				(Pop (1219uL, (Register "rbp")));
-				(Return 1220uL)
+		 		(Assign (1240uL, (Register "rsp"), (Register "rbp")));
+				(Pop (1241uL, (Register "rbp")));
+				(Return 1242uL)
 				]))
 		]
 let testprogram = mylambda 
-let make_callentry = [(MkCallentry 1200uL "main" [] Public false);(MkCallentry 1210uL "counter" [Mkintarg;Mkintarg] Public false)]
+let make_callentry = [(MkCallentry 1200uL "main" [] Public false);(MkCallentry 1230uL "counter" [Mkintarg;Mkintarg] Public false)]
 let make_calltable = 
 		   let calltabentry = make_callentry in
 			(MkCalltable calltabentry)
